AdequacySound compiles

proof/AdequacySound.v
@@ -40,20 +40,20 @@ Section ADQSOUND.
   Let skenv_link_tgt := sk_link_tgt.(Sk.load_skenv).
 
   (* stack can go preservation when su0 is given *)
-  Inductive sound_stack (su0: Sound.t) (args: Args.t) (m_arg: mem): list Frame.t -> Prop :=
+  Inductive sound_stack (su0: Sound.t) (args: Args.t): list Frame.t -> Prop :=
   | sound_stack_nil
     :
-      sound_stack su0 args m_arg []
+      sound_stack su0 args []
   | sound_stack_cons
-      su_tail m_tail args_tail tail
+      su_tail args_tail tail
       ms lst0
-      (TL: sound_stack su_tail args_tail m_tail tail)
+      (TL: sound_stack su_tail args_tail tail)
       (K: forall
           sound_state_all
           (PRSV: local_preservation ms sound_state_all)
         ,
-          (<<SUST: sound_state_all su0 m_arg lst0>>)
-          /\
+          (* (<<SUST: sound_state_all su0 args.(Args.m) lst0>>) *)
+          (* /\ *)
           (<<K: forall
               retv lst1
               su_greatest
@@ -62,7 +62,8 @@ Section ADQSOUND.
               (MLE: Sound.mle su_greatest args.(Args.m) retv.(Retv.m))
               (AFTER: ms.(ModSem.after_external) lst0 retv lst1)
             ,
-              sound_state_all su0 m_arg lst1>>)
+              (* sound_state_all su0 args.(Args.m) lst1>>) *)
+              sound_state_all su0 args_tail.(Args.m) lst1>>)
       )
       (GR: Sound.get_greatest args_tail su0)
       (EX: exists sound_state_ex, local_preservation ms sound_state_ex)
@@ -70,22 +71,23 @@ Section ADQSOUND.
       (* (PRSV: local_preservation ms sound_state_ex) *)
       (* (HD: sound_state_ex su0 lst0) *)
     :
-      sound_stack su0 args m_arg ((Frame.mk ms lst0) :: tail)
+      sound_stack su0 args ((Frame.mk ms lst0) :: tail)
   .
 
   Inductive sound_state (su0: Sound.t): mem -> state -> Prop :=
   | sound_state_normal
-      su_tail args_tail m_tail tail
+      su_tail args_tail tail
       ms lst0
       m_arg
       (GR: Sound.get_greatest args_tail su0)
-      (TL: sound_stack su_tail args_tail m_tail tail)
+      (TL: sound_stack su_tail args_tail tail)
       (HD: forall
           sound_state_all
           (PRSV: local_preservation ms sound_state_all)
         ,
           <<SUST: sound_state_all su0 m_arg lst0>>)
       (EX: exists sound_state_ex, local_preservation ms sound_state_ex)
+      (ABCD: args_tail.(Args.m) = m_arg)
     :
       sound_state su0 m_arg (State ((Frame.mk ms lst0) :: tail))
   | sound_state_call
@@ -93,7 +95,7 @@ Section ADQSOUND.
       args
       (GR: Sound.get_greatest args su0)
       (ARGS: Sound.args su0 args)
-      (STK: sound_stack su_tail args m_tail frs)
+      (STK: sound_stack su_tail args frs)
     :
       sound_state su0 m_tail (Callstate args frs)
   .
@@ -106,21 +108,23 @@ Section ADQSOUND.
   .
   Proof.
     inv INIT.
+    hexploit (Sound.greatest_ex (Args.mk (Genv.symbol_address (Sk.load_skenv sk_link) (prog_main sk_link) Ptrofs.zero)
+                                         []
+                                         m_init)); eauto. i; des.
     esplits; eauto. econs; s; eauto.
-    - admit "this should hold".
-    - eapply Sound.top_args.
+    - eapply Sound.greatest_spec; eauto.
     - econs; eauto.
   Unshelve.
+    all: ss.
     all: try exact Sound.top.
-    all: try exact Mem.empty.
   Qed.
 
   Lemma sound_progress
-        su0 st0 m_init0 tr st1
-        (SUST: sound_state su0 m_init0 st0)
+        su0 st0 m_arg0 tr st1
+        (SUST: sound_state su0 m_arg0 st0)
         (STEP: Step sem_src st0 tr st1)
     :
-      <<SUST: exists su1 m_init1, sound_state su1 m_init1 st1>>
+      <<SUST: exists su1 m_arg1, sound_state su1 m_arg1 st1>>
   .
   Proof.
     inv STEP.
@@ -128,18 +132,29 @@ Section ADQSOUND.
       inv SUST. ss.
       generalize (Sound.greatest_ex args). i; des.
       exists su_gr.
+      exists args.(Args.m).
       esplits; eauto.
       econs; eauto.
       { eapply Sound.greatest_spec; eauto. }
       econs; eauto.
-      ii.
-      dsplits; eauto.
-      inv PRSV. exploit CALL; eauto. i; des.
-      ii.
-      assert(su_greatest = su_gr0).
-      { eapply Sound.greatest_dtm; eauto. }
-      clarify.
-      eapply K; eauto.
+      {
+        ii. dup PRSV. bar. inv PRSV. exploit CALL; eauto; cycle 1.
+        { i; des.
+          assert(su_gr0 = su_greatest).
+          { eapply Sound.greatest_dtm; eauto. }
+          clarify.
+          eapply K; eauto.
+        }
+        eapply HD; eauto.
+      }
+      (* intros ? ?. *)
+      (* bar. dup PRSV. inv PRSV. bar. exploit CALL; eauto. { eapply HD; eauto. } i; des. *)
+      (* dsplits; eauto. *)
+      (* ii. *)
+      (* assert(su_greatest = su_gr0). *)
+      (* { eapply Sound.greatest_dtm; eauto. } *)
+      (* clarify. *)
+      (* eapply K; eauto. *)
     - (* INIT *)
       inv SUST. ss. des_ifs.
 
@@ -150,23 +165,15 @@ Section ADQSOUND.
         des; clarify.
         { eapply system_local_preservation. }
         u in MODSEM.
-        rewrite in_map_iff in MODSEM. des; clarify.
-        exploit SIMPROG.
-        { admit "somehow". }
-        i; des. inv H.
-        admit "somehow".
-      (* inv STK. *)
-      (* { esplits; eauto. econs; eauto. *)
-      (*   - econs; eauto. *)
-      (*   - ii. inv PRSV. dsplits; eauto. *)
-      (*     + ii. *)
-      (*       (* exploit CALL; eauto. *) *)
-      (*       admit "". *)
-      (* } *)
-      (* esplits; eauto. econs; eauto. econs; eauto. *)
-      (* { econs; eauto. } *)
-      (* i. inv PRSV. dsplits; eauto. *)
-      (* ii. exploit CALL; eauto. *)
+        rewrite in_map_iff in MODSEM. des; clarify. rename x into md_src.
+        assert(exists mp, In mp pp /\ mp.(ModPair.src) = md_src).
+        { clear - MODSEM0. rr in pp. rr in p_src. subst p_src. rewrite in_map_iff in *. des. eauto. }
+        des.
+        exploit SIMPROG; eauto. intros MPSIM. inv MPSIM.
+        exploit SIMMS.
+        { eapply SimSymb.le_refl. }
+        { admit "somehow. 1) fat module / skinny modsem. 2) require as premise". }
+        i; des. inv H0. ss. esplits; eauto.
     - (* INTERNAL *)
       inv SUST. ss.
       esplits; eauto. econs; eauto.
@@ -175,6 +182,7 @@ Section ADQSOUND.
       + split; ii; ModSem.tac.
     - (* RETURN *)
       inv SUST. ss. rename ms into ms_top.
+      rename args_tail into args_tail_top.
       bar.
       inv TL. ss.
       unfold Frame.update_st. s.
@@ -186,37 +194,9 @@ Section ADQSOUND.
       esplits; eauto. econs; try apply TL0; eauto.
       ii. specialize (K sound_state_all PRSV).
       eapply K; eauto.
-      rp; eauto.
   Unshelve.
-  Qed.
-      dup PRSV. inv PRSV.
-      exploit RET; ss; eauto.
-      exploit K; eauto. i; des.
-      eapply K0; eauto.
-      exploit RET; eauto.
-      { eapply HD; eauto. }
-      {
-      inv STK. inv TL.
-      esplits; eauto. econs; eauto. econs; eauto. ss.
-      assert(RETV: Sound.retv su0 retv).
-      { admit "". }
-      i. dup PRSV. inv PRSV.
-    - 
-    - (* INTERNAL *)
-      inv SUST. inv STK. ss.
-      esplits; eauto.
-      econs; eauto.
-      econs; eauto.
-      ss.
-      ii. dup PRSV. inv PRSV. eapply STEP; eauto.
-      + eapply HD; eauto.
-      + split; ii; ModSem.tac.
-    - (* RETURN *)
-      inv SUST. inv STK. inv TL.
-      esplits; eauto. econs; eauto. econs; eauto. ss.
-      assert(RETV: Sound.retv su0 retv).
-      { admit "". }
-      i. dup PRSV. inv PRSV.
+    all: ss.
+    admit "related to above admit".
   Qed.
 
 End ADQSOUND.
